Phi_System/Phi_Type_Algebra.thy
@@ -694,6 +694,9 @@ subsubsection \<open>Derived Rules\<close>
  and To_ToA_derived_Tr_functor = (60, [60,60]) for \<open>x \<Ztypecolon> T \<t>\<r>\<a>\<n>\<s>\<f>\<o>\<r>\<m>\<s> y \<Ztypecolon> U \<s>\<u>\<b>\<j> y. r x y \<w>\<i>\<t>\<h> P @action to U\<close>
                                                 in To_ToA_derived
     \<open>Derived To-Transformation rules for transformation functor\<close>
+  and To_ToA_derived_Tr_functor_fuzzy = (55, [55,55]) for \<open>x \<Ztypecolon> T \<t>\<r>\<a>\<n>\<s>\<f>\<o>\<r>\<m>\<s> y \<Ztypecolon> U \<s>\<u>\<b>\<j> y. r x y \<w>\<i>\<t>\<h> P @action to U\<close>
+                                                in To_ToA_derived and < To_ToA_derived_Tr_functor
+    \<open>when the annotated target \<phi>-type is in the element algebra but not the container\<close>
  and To_ToA_derived_to_raw = (60, [60,60]) for \<open>x \<Ztypecolon> T \<t>\<r>\<a>\<n>\<s>\<f>\<o>\<r>\<m>\<s> y \<Ztypecolon> Itself \<s>\<u>\<b>\<j> y. r x y \<w>\<i>\<t>\<h> P @action to Itself\<close>
                                             in To_ToA_derived
     \<open>Derived To-Transformation openning down the raw concrete representation\<close>
@@ -1693,6 +1696,17 @@ lemma [\<phi>reason_template default %To_ToA_derived_Tr_functor name Fa.To_Trans
 \<Longrightarrow> \<p>\<r>\<e>\<m>\<i>\<s>\<e> (\<forall>a b. a \<in> D x \<and> g a b \<longrightarrow> b \<in> R x)
 \<Longrightarrow> x \<Ztypecolon> Fa T \<t>\<r>\<a>\<n>\<s>\<f>\<o>\<r>\<m>\<s> y \<Ztypecolon> Fb U \<s>\<u>\<b>\<j> y. mapper g x y @action to (Fb Z) \<close>
   unfolding Action_Tag_def \<r>Guard_def
+  using transformation[unfolded \<r>Guard_def, where Fa=Fa and Fb=Fb and D=D and R=R and mapper=mapper] .
+
+lemma [\<phi>reason_template default %To_ToA_derived_Tr_functor_fuzzy name Fa.To_Transformation]:
+  \<open> NO_SIMP (\<g>\<u>\<a>\<r>\<d> NO_MATCH TYPE('c\<^sub>a\<^sub>a) TYPE('c))
+\<Longrightarrow> \<g>\<u>\<a>\<r>\<d> Transformation_Functor Fa Fb T U D R mapper
+\<Longrightarrow> (\<And>a \<in> D x. a \<Ztypecolon> T \<t>\<r>\<a>\<n>\<s>\<f>\<o>\<r>\<m>\<s> b \<Ztypecolon> U \<s>\<u>\<b>\<j> b. g a b @action to Z)
+\<Longrightarrow> \<p>\<r>\<e>\<m>\<i>\<s>\<e> (\<forall>a b. a \<in> D x \<and> g a b \<longrightarrow> b \<in> R x)
+\<Longrightarrow> x \<Ztypecolon> Fa T \<t>\<r>\<a>\<n>\<s>\<f>\<o>\<r>\<m>\<s> y \<Ztypecolon> Fb U \<s>\<u>\<b>\<j> y. mapper g x y @action to Z
+    <except-pattern> (XX::'c\<^sub>a\<^sub>a BI) \<t>\<r>\<a>\<n>\<s>\<f>\<o>\<r>\<m>\<s> YY \<w>\<i>\<t>\<h> PP @action to Z \<close>
+  for Fa :: \<open>('c\<^sub>a, 'a\<^sub>a) \<phi> \<Rightarrow> ('c,'a) \<phi>\<close> and Z :: \<open>('c\<^sub>a\<^sub>a, 'a\<^sub>a\<^sub>a) \<phi>\<close>
+  unfolding Action_Tag_def \<r>Guard_def Except_Pattern_def
   using transformation[unfolded \<r>Guard_def, where Fa=Fa and Fb=Fb and D=D and R=R and mapper=mapper] .
 
 lemma [\<phi>reason_template default %To_ToA_derived_Tr_functor name Fa.to_traverse]:
